src/c/include/coq-vsu-int_or_ptr/src/int_or_ptr.c
@@ -3,13 +3,11 @@
 
 #include "../int_or_ptr.h"
 
-/* The following functions should (in practice) compile correctly in CompCert,
-   but the CompCert correctness specification does not _require_ that
-   they compile correctly:  their semantics is "undefined behavior" in
-   CompCert C (and in C11), but in practice they will work in any compiler. */
-
 int int_or_ptr__is_int (int_or_ptr x) {
-    return (int)(((int_sizeofptr)x)&1);
+    if ((uint_sizeofptr)0 == (uint_sizeofptr)(((int_sizeofptr)x)&1)) {
+        return 0;
+    }
+    return 1;
 }
 
 int_sizeofptr int_or_ptr__to_int (int_or_ptr x) {
