theories/int_or_ptr/vst/clightgen/x86_32-linux/int_or_ptr.v
@@ -11,9 +11,9 @@ Module Info.
   Definition build_tag := "".
   Definition build_branch := "".
   Definition arch := "x86".
-  Definition model := "64".
+  Definition model := "32sse2".
   Definition abi := "standard".
-  Definition bitsize := 64.
+  Definition bitsize := 32.
   Definition big_endian := false.
   Definition source_file := "src/c/include/coq-vsu-int_or_ptr/src/int_or_ptr.c".
   Definition normalized := true.
@@ -86,59 +86,59 @@ Definition _x : ident := $"x".
 Definition f_int_or_ptr__is_int := {|
   fn_return := tint;
   fn_callconv := cc_default;
-  fn_params := ((_x, (talignas 3%N (tptr tvoid))) :: nil);
+  fn_params := ((_x, (talignas 2%N (tptr tvoid))) :: nil);
   fn_vars := nil;
   fn_temps := nil;
   fn_body :=
 (Ssequence
-  (Sifthenelse (Ebinop Oeq (Ecast (Econst_int (Int.repr 0) tint) tulong)
+  (Sifthenelse (Ebinop Oeq (Ecast (Econst_int (Int.repr 0) tint) tuint)
                  (Ecast
                    (Ebinop Oand
-                     (Ecast (Etempvar _x (talignas 3%N (tptr tvoid))) tlong)
-                     (Econst_int (Int.repr 1) tint) tlong) tulong) tint)
+                     (Ecast (Etempvar _x (talignas 2%N (tptr tvoid))) tint)
+                     (Econst_int (Int.repr 1) tint) tint) tuint) tint)
     (Sreturn (Some (Econst_int (Int.repr 0) tint)))
     Sskip)
   (Sreturn (Some (Econst_int (Int.repr 1) tint))))
 |}.
 
 Definition f_int_or_ptr__to_int := {|
-  fn_return := tlong;
+  fn_return := tint;
   fn_callconv := cc_default;
-  fn_params := ((_x, (talignas 3%N (tptr tvoid))) :: nil);
+  fn_params := ((_x, (talignas 2%N (tptr tvoid))) :: nil);
   fn_vars := nil;
   fn_temps := nil;
   fn_body :=
-(Sreturn (Some (Ecast (Etempvar _x (talignas 3%N (tptr tvoid))) tlong)))
+(Sreturn (Some (Ecast (Etempvar _x (talignas 2%N (tptr tvoid))) tint)))
 |}.
 
 Definition f_int_or_ptr__to_ptr := {|
   fn_return := (tptr tvoid);
   fn_callconv := cc_default;
-  fn_params := ((_x, (talignas 3%N (tptr tvoid))) :: nil);
+  fn_params := ((_x, (talignas 2%N (tptr tvoid))) :: nil);
   fn_vars := nil;
   fn_temps := nil;
   fn_body :=
-(Sreturn (Some (Ecast (Etempvar _x (talignas 3%N (tptr tvoid))) (tptr tvoid))))
+(Sreturn (Some (Ecast (Etempvar _x (talignas 2%N (tptr tvoid))) (tptr tvoid))))
 |}.
 
 Definition f_int_or_ptr__of_int := {|
-  fn_return := (talignas 3%N (tptr tvoid));
+  fn_return := (talignas 2%N (tptr tvoid));
   fn_callconv := cc_default;
-  fn_params := ((_x, tlong) :: nil);
+  fn_params := ((_x, tint) :: nil);
   fn_vars := nil;
   fn_temps := nil;
   fn_body :=
-(Sreturn (Some (Ecast (Etempvar _x tlong) (talignas 3%N (tptr tvoid)))))
+(Sreturn (Some (Ecast (Etempvar _x tint) (talignas 2%N (tptr tvoid)))))
 |}.
 
 Definition f_int_or_ptr__of_ptr := {|
-  fn_return := (talignas 3%N (tptr tvoid));
+  fn_return := (talignas 2%N (tptr tvoid));
   fn_callconv := cc_default;
   fn_params := ((_x, (tptr tvoid)) :: nil);
   fn_vars := nil;
   fn_temps := nil;
   fn_body :=
-(Sreturn (Some (Ecast (Etempvar _x (tptr tvoid)) (talignas 3%N (tptr tvoid)))))
+(Sreturn (Some (Ecast (Etempvar _x (tptr tvoid)) (talignas 2%N (tptr tvoid)))))
 |}.
 
 Definition composites : list composite_definition :=
@@ -147,7 +147,7 @@ nil.
 Definition global_definitions : list (ident * globdef fundef type) :=
 ((___builtin_ais_annot,
    Gfun(External (EF_builtin "__builtin_ais_annot"
-                   (mksignature (AST.Tlong :: nil) AST.Tvoid
+                   (mksignature (AST.Tint :: nil) AST.Tvoid
                      {|cc_vararg:=(Some 1); cc_unproto:=false; cc_structret:=false|}))
      (Tcons (tptr tschar) Tnil) tvoid
      {|cc_vararg:=(Some 1); cc_unproto:=false; cc_structret:=false|})) ::
@@ -173,8 +173,8 @@ Definition global_definitions : list (ident * globdef fundef type) :=
      (Tcons tuint Tnil) tint cc_default)) ::
  (___builtin_clzl,
    Gfun(External (EF_builtin "__builtin_clzl"
-                   (mksignature (AST.Tlong :: nil) AST.Tint cc_default))
-     (Tcons tulong Tnil) tint cc_default)) ::
+                   (mksignature (AST.Tint :: nil) AST.Tint cc_default))
+     (Tcons tuint Tnil) tint cc_default)) ::
  (___builtin_clzll,
    Gfun(External (EF_builtin "__builtin_clzll"
                    (mksignature (AST.Tlong :: nil) AST.Tint cc_default))
@@ -185,8 +185,8 @@ Definition global_definitions : list (ident * globdef fundef type) :=
      (Tcons tuint Tnil) tint cc_default)) ::
  (___builtin_ctzl,
    Gfun(External (EF_builtin "__builtin_ctzl"
-                   (mksignature (AST.Tlong :: nil) AST.Tint cc_default))
-     (Tcons tulong Tnil) tint cc_default)) ::
+                   (mksignature (AST.Tint :: nil) AST.Tint cc_default))
+     (Tcons tuint Tnil) tint cc_default)) ::
  (___builtin_ctzll,
    Gfun(External (EF_builtin "__builtin_ctzll"
                    (mksignature (AST.Tlong :: nil) AST.Tint cc_default))
@@ -210,10 +210,10 @@ Definition global_definitions : list (ident * globdef fundef type) :=
  (___builtin_memcpy_aligned,
    Gfun(External (EF_builtin "__builtin_memcpy_aligned"
                    (mksignature
-                     (AST.Tlong :: AST.Tlong :: AST.Tlong :: AST.Tlong ::
-                      nil) AST.Tvoid cc_default))
+                     (AST.Tint :: AST.Tint :: AST.Tint :: AST.Tint :: nil)
+                     AST.Tvoid cc_default))
      (Tcons (tptr tvoid)
-       (Tcons (tptr tvoid) (Tcons tulong (Tcons tulong Tnil)))) tvoid
+       (Tcons (tptr tvoid) (Tcons tuint (Tcons tuint Tnil)))) tvoid
      cc_default)) ::
  (___builtin_sel,
    Gfun(External (EF_builtin "__builtin_sel"
@@ -223,13 +223,13 @@ Definition global_definitions : list (ident * globdef fundef type) :=
      {|cc_vararg:=(Some 1); cc_unproto:=false; cc_structret:=false|})) ::
  (___builtin_annot,
    Gfun(External (EF_builtin "__builtin_annot"
-                   (mksignature (AST.Tlong :: nil) AST.Tvoid
+                   (mksignature (AST.Tint :: nil) AST.Tvoid
                      {|cc_vararg:=(Some 1); cc_unproto:=false; cc_structret:=false|}))
      (Tcons (tptr tschar) Tnil) tvoid
      {|cc_vararg:=(Some 1); cc_unproto:=false; cc_structret:=false|})) ::
  (___builtin_annot_intval,
    Gfun(External (EF_builtin "__builtin_annot_intval"
-                   (mksignature (AST.Tlong :: AST.Tint :: nil) AST.Tint
+                   (mksignature (AST.Tint :: AST.Tint :: nil) AST.Tint
                      cc_default)) (Tcons (tptr tschar) (Tcons tint Tnil))
      tint cc_default)) ::
  (___builtin_membar,
@@ -238,38 +238,38 @@ Definition global_definitions : list (ident * globdef fundef type) :=
      cc_default)) ::
  (___builtin_va_start,
    Gfun(External (EF_builtin "__builtin_va_start"
-                   (mksignature (AST.Tlong :: nil) AST.Tvoid cc_default))
+                   (mksignature (AST.Tint :: nil) AST.Tvoid cc_default))
      (Tcons (tptr tvoid) Tnil) tvoid cc_default)) ::
  (___builtin_va_arg,
    Gfun(External (EF_builtin "__builtin_va_arg"
-                   (mksignature (AST.Tlong :: AST.Tint :: nil) AST.Tvoid
+                   (mksignature (AST.Tint :: AST.Tint :: nil) AST.Tvoid
                      cc_default)) (Tcons (tptr tvoid) (Tcons tuint Tnil))
      tvoid cc_default)) ::
  (___builtin_va_copy,
    Gfun(External (EF_builtin "__builtin_va_copy"
-                   (mksignature (AST.Tlong :: AST.Tlong :: nil) AST.Tvoid
+                   (mksignature (AST.Tint :: AST.Tint :: nil) AST.Tvoid
                      cc_default))
      (Tcons (tptr tvoid) (Tcons (tptr tvoid) Tnil)) tvoid cc_default)) ::
  (___builtin_va_end,
    Gfun(External (EF_builtin "__builtin_va_end"
-                   (mksignature (AST.Tlong :: nil) AST.Tvoid cc_default))
+                   (mksignature (AST.Tint :: nil) AST.Tvoid cc_default))
      (Tcons (tptr tvoid) Tnil) tvoid cc_default)) ::
  (___compcert_va_int32,
    Gfun(External (EF_external "__compcert_va_int32"
-                   (mksignature (AST.Tlong :: nil) AST.Tint cc_default))
+                   (mksignature (AST.Tint :: nil) AST.Tint cc_default))
      (Tcons (tptr tvoid) Tnil) tuint cc_default)) ::
  (___compcert_va_int64,
    Gfun(External (EF_external "__compcert_va_int64"
-                   (mksignature (AST.Tlong :: nil) AST.Tlong cc_default))
+                   (mksignature (AST.Tint :: nil) AST.Tlong cc_default))
      (Tcons (tptr tvoid) Tnil) tulong cc_default)) ::
  (___compcert_va_float64,
    Gfun(External (EF_external "__compcert_va_float64"
-                   (mksignature (AST.Tlong :: nil) AST.Tfloat cc_default))
+                   (mksignature (AST.Tint :: nil) AST.Tfloat cc_default))
      (Tcons (tptr tvoid) Tnil) tdouble cc_default)) ::
  (___compcert_va_composite,
    Gfun(External (EF_external "__compcert_va_composite"
-                   (mksignature (AST.Tlong :: AST.Tlong :: nil) AST.Tlong
-                     cc_default)) (Tcons (tptr tvoid) (Tcons tulong Tnil))
+                   (mksignature (AST.Tint :: AST.Tint :: nil) AST.Tint
+                     cc_default)) (Tcons (tptr tvoid) (Tcons tuint Tnil))
      (tptr tvoid) cc_default)) ::
  (___builtin_unreachable,
    Gfun(External (EF_builtin "__builtin_unreachable"
@@ -277,8 +277,8 @@ Definition global_definitions : list (ident * globdef fundef type) :=
      cc_default)) ::
  (___builtin_expect,
    Gfun(External (EF_builtin "__builtin_expect"
-                   (mksignature (AST.Tlong :: AST.Tlong :: nil) AST.Tlong
-                     cc_default)) (Tcons tlong (Tcons tlong Tnil)) tlong
+                   (mksignature (AST.Tint :: AST.Tint :: nil) AST.Tint
+                     cc_default)) (Tcons tint (Tcons tint Tnil)) tint
      cc_default)) ::
  (___compcert_i64_dtos,
    Gfun(External (EF_runtime "__compcert_i64_dtos"
@@ -389,21 +389,21 @@ Definition global_definitions : list (ident * globdef fundef type) :=
      cc_default)) ::
  (___builtin_read16_reversed,
    Gfun(External (EF_builtin "__builtin_read16_reversed"
-                   (mksignature (AST.Tlong :: nil) AST.Tint16unsigned
+                   (mksignature (AST.Tint :: nil) AST.Tint16unsigned
                      cc_default)) (Tcons (tptr tushort) Tnil) tushort
      cc_default)) ::
  (___builtin_read32_reversed,
    Gfun(External (EF_builtin "__builtin_read32_reversed"
-                   (mksignature (AST.Tlong :: nil) AST.Tint cc_default))
+                   (mksignature (AST.Tint :: nil) AST.Tint cc_default))
      (Tcons (tptr tuint) Tnil) tuint cc_default)) ::
  (___builtin_write16_reversed,
    Gfun(External (EF_builtin "__builtin_write16_reversed"
-                   (mksignature (AST.Tlong :: AST.Tint :: nil) AST.Tvoid
+                   (mksignature (AST.Tint :: AST.Tint :: nil) AST.Tvoid
                      cc_default)) (Tcons (tptr tushort) (Tcons tushort Tnil))
      tvoid cc_default)) ::
  (___builtin_write32_reversed,
    Gfun(External (EF_builtin "__builtin_write32_reversed"
-                   (mksignature (AST.Tlong :: AST.Tint :: nil) AST.Tvoid
+                   (mksignature (AST.Tint :: AST.Tint :: nil) AST.Tvoid
                      cc_default)) (Tcons (tptr tuint) (Tcons tuint Tnil))
      tvoid cc_default)) ::
  (___builtin_debug,
