theories/int_or_ptr/vst/spec/spec.v
@@ -2,32 +2,21 @@ From VST Require Import floyd.proofauto.
 
 From appliedfm Require Import int_or_ptr.model.int_or_ptr.
 From appliedfm Require Import int_or_ptr.vst.ast.ast.
+From appliedfm Require Import int_or_ptr.vst.cmodel.val.
 From appliedfm Require Import int_or_ptr.vst.clightgen.int_or_ptr.
-
-Definition valid_int_or_ptr (x: val) :=
-  match x with
-  | Vint i => if Archi.ptr64 then False else Int.testbit i 0 = true
-  | Vptr _ z => Ptrofs.testbit z 0 = false /\ Ptrofs.testbit z 1 = false
-  | Vlong i => if Archi.ptr64 then Int64.testbit i 0 = true else False
-  | _ => False
-  end.
 
 Definition int_or_ptr__is_int_spec :=
  DECLARE _int_or_ptr__is_int
  WITH x : val
  PRE [ int_or_ptr_type ]
-   PROP (valid_int_or_ptr x)
+   PROP (int_or_ptr__is_valid x)
    PARAMS (x)
    GLOBALS ()
    SEP ()
  POST [ tint ]
    PROP()
    LOCAL(temp ret_temp
-          (Vint (Int.repr (match x with
-                           | Vint _ => if Archi.ptr64 then 0 else 1
-                           | Vlong _ => if Archi.ptr64 then 1 else 0
-                           | _ => 0
-                           end))))
+          (Vint (Int.repr (if (int_or_ptr__is_int x) then 1 else 0))))
    SEP().
 
 Definition int_or_ptr__to_int_spec :=
@@ -56,7 +45,7 @@ Definition int_or_ptr__of_int_spec :=
   DECLARE _int_or_ptr__of_int
   WITH x : val
   PRE [ (if Archi.ptr64 then tlong else tint) ]
-    PROP (valid_int_or_ptr x)
+    PROP (int_or_ptr__is_valid x)
     PARAMS (x)
     GLOBALS ()
     SEP ()
@@ -67,9 +56,17 @@ Definition int_or_ptr__of_ptr_spec :=
   DECLARE _int_or_ptr__of_ptr
   WITH x : val
   PRE [ tptr tvoid ]
-    PROP (valid_int_or_ptr x)
+    PROP (int_or_ptr__is_valid x)
     PARAMS (x)
     GLOBALS ()
     SEP()
   POST [ int_or_ptr_type ]
     PROP() LOCAL (temp ret_temp x) SEP().
+
+Definition ASI: funspecs := ltac:(with_library prog
+  [ int_or_ptr__is_int_spec
+  ; int_or_ptr__to_int_spec
+  ; int_or_ptr__to_ptr_spec
+  ; int_or_ptr__of_int_spec
+  ; int_or_ptr__of_ptr_spec
+  ]).
