theories/int_or_ptr/vst/cmodel/val.v
@@ -1,0 +1,41 @@
+From Coq Require Import ZArith.ZArith.
+
+From compcert Require Import common.Values.
+From compcert Require Import lib.Integers.
+
+Local Open Scope Z.
+
+Definition int_or_ptr__is_valid_int (x: val): Prop :=
+  if Archi.ptr64
+  then
+    match x with
+    | Vlong i => Int64.testbit i 0 = true
+    | _ => False
+    end
+  else
+    match x with
+    | Vint i => Int.testbit i 0 = true
+    | _ => False
+    end.
+
+Definition int_or_ptr__is_valid_ptr (x: val): Prop :=
+  match x with
+  | Vptr _ z => Ptrofs.testbit z 0 = false /\ Ptrofs.testbit z 1 = false
+  | _ => False
+  end.
+
+Definition int_or_ptr__is_valid (x: val): Prop :=
+  int_or_ptr__is_valid_int x \/ int_or_ptr__is_valid_ptr x.
+
+Definition int_or_ptr__is_int (x: val): bool
+ := if Archi.ptr64
+    then
+      match x with
+      | Vlong _ => true
+      | _ => false
+      end
+    else
+      match x with
+      | Vint _ => true
+      | _ => false
+      end.
