theories/int_or_ptr/vst/verif/verif.v
@@ -1,0 +1,88 @@
+From VST Require Import floyd.proofauto.
+
+From appliedfm Require Import int_or_ptr.model.int_or_ptr.
+From appliedfm Require Import int_or_ptr.vst.ast.ast.
+From appliedfm Require Import int_or_ptr.vst.clightgen.int_or_ptr.
+From appliedfm Require Import int_or_ptr.vst.cmodel.val.
+From appliedfm Require Import int_or_ptr.vst.spec.spec.
+
+Lemma body_int_or_ptr__is_int:
+  semax_body Vprog ASI f_int_or_ptr__is_int int_or_ptr__is_int_spec.
+Proof.
+  start_function.
+  forward_if.
+  {
+    destruct H as [H|H].
+    - destruct x ; simpl in H ; try contradiction.
+      unfold denote_tc_islong, denote_tc_isint.
+      unfold is_long, is_int.
+      entailer!.
+    - destruct x ; simpl in * ; try contradiction.
+      subst v.
+      simpl in *.
+      (* this is ... not so true *)
+      admit.
+  }
+  {
+    forward.
+    entailer!.
+    change (Tpointer Tvoid {| attr_volatile := false; attr_alignas := Some 3%N |}) with int_or_ptr_type in H1.
+    change (Tpointer Tvoid {| attr_volatile := false; attr_alignas := Some 2%N |}) with int_or_ptr_type in H1.
+    simpl in H1.
+    destruct H as [H|H] ; destruct x ; simpl in * ; try easy.
+    exfalso.
+    change
+      (Int64.repr (Int.signed (Int.repr 1)))
+      with (Int64.repr 1)
+      in H0.
+    first
+      [ replace
+          (Int64.and i (Int64.repr 1))
+          with (Int64.repr 1)
+          in H0
+      | replace
+          (Int.and i (Int.repr 1))
+          with (Int.repr 1)
+          in H0
+      ].
+    {
+      now cbv in H0.
+    }
+    clear -H.
+    unfold int_or_ptr__is_valid_int in H.
+    (* this is actually true *)
+    admit.
+  }
+  forward.
+  entailer!.
+  destruct H as [H|H] ; now destruct x.
+Admitted.
+
+Lemma body_int_or_ptr__of_int:
+  semax_body Vprog ASI f_int_or_ptr__of_int int_or_ptr__of_int_spec.
+Proof.
+  start_function.
+  forward.
+Qed.
+
+Lemma body_int_or_ptr__to_int:
+  semax_body Vprog ASI f_int_or_ptr__to_int int_or_ptr__to_int_spec.
+Proof.
+  start_function.
+  red in H. destruct x; try easy.
+  forward.
+Qed.
+
+Lemma body_int_or_ptr__of_ptr:
+  semax_body Vprog ASI f_int_or_ptr__of_ptr int_or_ptr__of_ptr_spec.
+Proof.
+  start_function.
+  forward.
+Qed.
+
+Lemma body_int_or_ptr__to_ptr:
+  semax_body Vprog ASI f_int_or_ptr__to_ptr int_or_ptr__to_ptr_spec.
+Proof.
+  start_function.
+  forward.
+Qed.
